polymorphic map done

compositionality/Polymorphic_gmap/Polymorphic_gmap.fst
@@ -10,17 +10,13 @@ let init_st_a = 0
 
 let init_st_b = S.empty
 
-let symmetric_a a b = ()
+let eq_a a b = a = b
 
-let symmetric_b a b = ()
+let eq_b a b = S.equal a b
 
-let transitive_a a b c = ()
+let lem_eq_a a b = ()
 
-let transitive_b a b c = ()
-
-let eq_is_equiv_a a b = ()
-
-let eq_is_equiv_b a b = ()
+let lem_eq_b a b = ()
 
 type app_op_a : eqtype =
   |Inc
@@ -45,17 +41,6 @@ let merge_b l a b = S.union l (S.union a b)
 
 /////////////////////////////////////////////////////////////////////////////
 
-let lem_eq (a b:concrete_st)
-  : Lemma (requires (forall k. S.equal (sel a (Beta_t k)) (sel b (Beta_t k)) /\ (sel a (Alpha_t k) == sel b (Alpha_t k))) /\
-                    (forall k. M.contains a k = M.contains b k))
-          (ensures eq a b)
-          [SMTPat (eq a b)] = ()
-
-let lem_eq_b (a b:concrete_st_b)
-  : Lemma (requires S.equal a b)
-          (ensures eq_b a b)
-          [SMTPat (eq_b a b)] = ()
-
 #set-options "--ifuel 3"
 let rc_non_comm o1 o2 = ()
 let no_rc_chain o1 o2 o3 = ()
@@ -65,12 +50,9 @@ let cond_comm_ind s o1 o2 o3 o l = ()
 ////////////////////////////////////////////////////////////////////////////
 
 let merge_comm_a l a b = ()
-let merge_comm_b l a b = 
-  ()//assert (S.equal (S.union l (S.union a b)) (S.union l (S.union b a))); ()
-
+let merge_comm_b l a b = ()
 let merge_idem_a s = ()
-let merge_idem_b s = 
-  ()//assert (S.equal (S.union s (S.union s s)) s); ()
+let merge_idem_b s = ()
 
 ////////////////////////////////////////////////////////////////////////////
 
@@ -109,27 +91,19 @@ let rc_inter_lca_b l a b c o1 o2 ol oi = ()
 let rc_inter_lca_ne l a b c o1 o2 ol oi = ()
 
 let one_op_ind_right_a l a b o2 o2' = ()
-
-let one_op_ind_right_b l a b o2 o2' =
-  ()//assert (S.equal (S.union l (S.union a (do_b (do_b b o2') o2))) (do_b (S.union l (S.union a (do_b b o2'))) o2)); ()
-
+let one_op_ind_right_b l a b o2 o2' = ()
 let one_op_ind_right_ne l a b o2 o2' = ()
 
 let one_op_ind_left_a l a b o1 o1' = ()
-let one_op_ind_left_b l a b o1 o1' = 
-  () //assert (S.equal (S.union l (S.union (do_b (do_b a o1') o1) b)) (do_b (S.union l (S.union (do_b a o1') b)) o1)); ()
-  
+let one_op_ind_left_b l a b o1 o1' = ()
 let one_op_ind_left_ne l a b o1 o1' = ()
 
 let one_op_ind_lca_a l o2 o = ()
-let one_op_ind_lca_b l o2 o = 
-  () //assert (S.equal (S.union (do_b l o) (S.union (do_b l o) (do_b (do_b l o) o2))) (do_b (do_b l o) o2)); ()
-  
+let one_op_ind_lca_b l o2 o = ()
 let one_op_ind_lca_ne l o2 o = ()
 
 let one_op_base_a o2 = ()
-let one_op_base_b o2 = 
-  () //assert (S.equal (S.union init_st_b (S.union init_st_b (do_b init_st_b o2))) (do_b init_st_b o2)); ()
+let one_op_base_b o2 = ()
 
 let one_op_inter_base_right_a l a b c o2 ob ol = ()
 let one_op_inter_base_right_b l a b c o2 ob ol = ()
@@ -175,22 +149,16 @@ let zero_op_inter_lca_v2_b l a b c ol oi = ()
 let zero_op_inter_lca_v2_ne l a b c ol oi = ()
 
 let comm_ind_right_a l a b o1 o2 o2' = ()
-let comm_ind_right_b l a b o1 o2 o2' = 
-  ()//assert (S.equal (S.union l (S.union (do_b a o1) (do_b (do_b b o2') o2))) (do_b (do_b (merge_b l a (do_b b o2')) o2) o1)); ()
-
-#set-options "--z3rlimit 100 --ifuel 3"
+let comm_ind_right_b l a b o1 o2 o2' = ()
+#set-options "--z3rlimit 50"
 let comm_ind_right_ne l a b o1 o2 o2' = ()
 
 let comm_ind_left_a l a b o1 o2 o1' = ()
-let comm_ind_left_b l a b o1 o2 o1' = 
-  () //assert (S.equal (S.union l (S.union (do_b (do_b a o1') o1) (do_b b o2))) (do_b (do_b (merge_b l (do_b a o1') b) o2) o1)); ()
-  
+let comm_ind_left_b l a b o1 o2 o1' = ()
 let comm_ind_left_ne l a b o1 o2 o1' = ()
 
 let comm_ind_lca_a l ol o1 o2 = ()
-let comm_ind_lca_b l ol o1 o2 = 
-  () //assert (S.equal (S.union (do_b l ol) (S.union (do_b (do_b l ol) o1) (do_b (do_b l ol) o2))) (do_b (do_b (do_b l ol) o2) o1)); ()
-  
+let comm_ind_lca_b l ol o1 o2 = ()
 let comm_ind_lca_ne l ol o1 o2 = ()
 
 let comm_base o1 o2 t = ()
